test if an induction principle on denote is useful
Export some lemmas

add provide notation

Remove exports inside the framework.
Introduce notations for Provide and MayProvide and rework proofs around those.
Remove Generalizable All Variables (antipattern).

examples/airlock.v
@@ -4,19 +4,14 @@
 
 (* Copyright (C) 2018–2020 ANSSI *)
 
-From FreerDPS Require Import Init.
+From HB Require Import structures.
+From mathcomp Require Import all_boot classical_sets boolp.
+From monae Require Import hierarchy.
 (* WARNING: Move this import to its MathComp counterpart. *)
 From Stdlib Require Import Arith.
-From mathcomp Require Import all_boot classical_sets.
-From FreerDPS Require Import Core Freer Hoare.
+From FreerDPS Require Import Core.
 
 Import FreerFuns.
-Generalizable All Variables.
-
-
-(** * Specifying *)
-(* Opaque denote. *)
-
 
 Module Export DoorsControllerM.
 (** ** Doors *)
@@ -30,25 +25,24 @@ Inductive DOORS : effect :=
 | Toggle : door -> DOORS unit.
 
 Section doors_s.
-Context `{Provide Fx DOORS} {im : freerMonad Fx}.
+Context {Fx : effect} `{DOORS -< Fx} {M : freerMonad Fx}.
 
-Definition is_open (d : door) : im bool := trigger $ IsOpen d.
-Definition toggle (d : door) : im unit := trigger $ Toggle d.
-Definition open_door (d : door) : im unit :=
+Definition is_open (d : door) : M bool := trigger $ IsOpen d.
+Definition toggle (d : door) : M unit := trigger $ Toggle d.
+Definition open_door (d : door) : M unit :=
   is_open d >>= fun open => when (~~ open) (toggle d).
-Definition close_door (d : door) : im unit :=
+Definition close_door (d : door) : M unit :=
   is_open d >>= (when ^~ (toggle d)).
 End doors_s.
-(** ** Controller *)
 
 Inductive CONTROLLER : effect :=
 | Tick : CONTROLLER unit
 | RequestOpen (d : door) : CONTROLLER unit.
 
 Section controller_s.
-Context `{Provide Fx CONTROLLER} {im : freerMonad Fx}.
-Definition tick : im unit := trigger Tick.
-Definition request_open (d : door) : im unit := trigger $ RequestOpen d.
+Context {Fx : effect} `{CONTROLLER -< Fx} {M : freerMonad Fx}.
+Definition tick : M unit := trigger Tick.
+Definition request_open (d : door) : M unit := trigger $ RequestOpen d.
 End controller_s.
 
 Definition co (d : door) : door :=
@@ -60,8 +54,8 @@ Definition co (d : door) : door :=
 Lemma co_leftE : co left = right.
 Proof. by []. Qed.
 
-Definition controller `{Provide Fx DOORS, Provide Fx (STORE nat)}
-    {im : freerMonad Fx} : component (im:=im) CONTROLLER Fx :=
+Definition controller {Fx : effect} `{DOORS -< Fx, (STORE nat) -< Fx}
+    {M : freerMonad Fx} : component (M:=M) CONTROLLER Fx :=
   fun _ op =>
     match op with
     | Tick =>
@@ -125,7 +119,7 @@ Definition step (ω : Ω) (a : Type) (op : DOORS a) (_ : a) : Ω :=
   if op is Toggle d then tog d ω else ω.
 
 (** *** Requirements / Precondition *)
-Inductive doors_o_caller : Ω -> forall (a : Type), DOORS a -> Prop :=
+Inductive doors_o_caller : Ω -> forall (a : Type), set $ DOORS a :=
 (** - Given the door [d] of o system [ω], it is always possible to ask for the
       state of [d]. *)
 | req_is_open (d : door) (ω : Ω)
@@ -146,102 +140,16 @@ Inductive doors_o_callee : Ω -> forall (a : Type), DOORS a -> a -> Prop :=
 | doors_o_callee_toggle (d : door) (ω : Ω) (x : unit)
   : doors_o_callee ω unit (Toggle d) x.
 
+Lemma doors_o_callee_is_openE
+    {ω : Ω} {d : door} {opened : bool} :
+  doors_o_callee ω bool (IsOpen d) opened ->
+  sel d ω = opened.
+Proof. by inversion 1;ssubst. Qed.
+
 (* doors_c => {{door_caller}} p%step {{door_callee}} *)
 Definition doors_c : contract DOORS Ω :=
   make_contract step doors_o_caller doors_o_callee.
 (* -------------------------------------------------------------------------- *)
-
-Section doors_pre_post_helpers.
-Context `{Provide Fx DOORS} {a : Type}.
-
-Lemma doors_effect_preE (op : Fx a) (ω : Ω) :
-  pre (hoare_of_contract doors_c op) ω <->
-  match proj_p op with
-  | Some door_op => doors_o_caller ω a door_op
-  | None => True
-  end.
-Proof. by rewrite /hoare_of_contract /= /gen_caller_obligation. Qed.
-
-Lemma doors_effect_postE
-    (op : Fx a) (ω : Ω) (x : a) (ω' : Ω) :
-  post (hoare_of_contract doors_c op) ω x ω' <->
-  match proj_p op with
-  | Some door_op =>
-      ω' = step ω a door_op x /\ doors_o_callee ω a door_op x
-  | None => ω' = ω
-  end.
-Proof.
-rewrite /hoare_of_contract /= /gen_witness_update
-  /gen_callee_obligation.
-case: (proj_p op)=> [door_op |] /=.
-- by [].
-by split=> [[-> _] | ->].
-Qed.
-
-Lemma doors_pre_condE
-    (ω : Ω) (op : DOORS a) :
-  pre (hoare_of_contract doors_c (inj_p op)) ω <->
-  doors_o_caller ω a op.
-Proof. by rewrite doors_effect_preE proj_inj_p_equ. Qed.
-
-Lemma doors_post_condE
-    (ω : Ω) (op : DOORS a) (x : a) (ω' : Ω) :
-  post (hoare_of_contract doors_c (inj_p op)) ω x ω' <->
-  ω' = step ω a op x /\ doors_o_callee ω a op x.
-Proof. by rewrite doors_effect_postE proj_inj_p_equ. Qed.
-End doors_pre_post_helpers.
-
-Opaque hoare_of_contract.
-
-(*--------------------------- Intermediary Lemmas ----------------------------*)
-Section IntermLemmaS.
-Context `{Provide Fx DOORS} (ω : Ω) (d : door).
-
-Lemma doors_is_open_post_retE (opened : bool) (ω' : Ω) :
-  post (hoare_of_contract doors_c
-          (A := bool) (inj_p (IsOpen d))) ω opened ω' <->
-  post (@ret (hoare Ω) bool (sel d ω)) ω opened ω'.
-Proof.
-rewrite doors_post_condE;
-  split=> [ [-> callee] | [<- <-] ];
-  split=> //.
-- by inversion callee; ssubst.
-- exact: doors_o_callee_is_open.
-Qed.
-
-Lemma doors_is_open_preE :
-  pre (hoare_of_contract doors_c
-          (A := bool) (inj_p (IsOpen d))) ω <->
-  pre (@ret (hoare Ω) bool (sel d ω)) ω.
-Proof.
-by split=> // _;
-  rewrite doors_pre_condE;
-  exact: req_is_open.
-Qed.
-
-Lemma doors_toggle_postE (u : unit) (ω' : Ω) :
-  post (hoare_of_contract doors_c
-          (A := unit) (inj_p (Toggle d))) ω u ω' <->
-  ω' = tog d ω.
-Proof.
-by rewrite doors_post_condE;
-  split=> [ [-> _] | ->] //; split=>//;
-  exact: doors_o_callee_toggle.
-Qed.
-
-Lemma doors_toggle_preE
-    (* Safe means : door 1 is closed -> door 2 is closed *)
-    (* Previous: (safe : sel d ω = false -> sel (co d) ω = false) *)
-    (safe : sel (co d) ω -> sel d ω) :
-  pre (hoare_of_contract doors_c
-          (A := unit) (inj_p (Toggle d))) ω <->
-  pre (@ret (hoare Ω) unit tt) ω.
-Proof.
-by split=> // _;
-  rewrite doors_pre_condE;
-  exact: req_toggle safe.
-Qed.
-End IntermLemmaS.
 
 Local Open Scope classical_set_scope.
 
@@ -255,48 +163,48 @@ Qed.
 Definition doors_safe (ω : Ω) := ~~ sel left ω \/ ~~ sel right ω.
 
 Section RespectfulAndRunLemmas.
-Context `{Provide Fx DOORS} {im : freerMonad Fx}.
-Local Notation "p ||> c" := (to_hoare (im:=im) c p)
+Context {Fx : effect} `{DOORS -< Fx} {M : freerMonad Fx}.
+Local Notation "c ||> p" :=
+  (to_hoare (M:=M) c p)
   (at level 50, no associativity).
 
 (** Closing a door [d] in any system [ω] is always a respectful operation. *)
 Lemma close_door_respectful (d : door) :
-  pre (close_door d ||> doors_c) = [set: _].
+  pre (doors_c ||> close_door d) = [set: _].
 Proof.
-rewrite /close_door -subTset=> ω _; apply: th_pre_bindA.
-- by rewrite to_hoare_requestE doors_is_open_preE.
+rewrite /close_door -subTset=> hω _; apply: th_pre_bindA.
+- by rewrite to_hoare_trigger_preE; exact: req_is_open.
 case=> ?;
-  rewrite to_hoare_when_preE // to_hoare_requestE doors_is_open_post_retE
-  => -[? <-].
-by rewrite to_hoare_requestE;
-  apply/(doors_toggle_preE ω d).
+  rewrite to_hoare_when_preE // to_hoare_trigger_postE
+    => -[ /[swap] ]=>/doors_o_callee_is_openE ? -> .
+by rewrite to_hoare_trigger_preE;
+  apply: req_toggle.
 Qed.
 
 Lemma open_door_respectful (ω : Ω) (d : door) (safe : ~~ sel (co d) ω) :
-  pre (open_door d ||> doors_c) ω.
+  pre (doors_c ||> open_door d) ω.
 Proof.
 rewrite /open_door; apply: th_pre_bindA.
-- by rewrite to_hoare_requestE doors_is_open_preE.
+- by rewrite to_hoare_trigger_preE; exact: req_is_open.
 case=> ?;
-  rewrite to_hoare_when_preE // to_hoare_requestE doors_is_open_post_retE
-  => -[_ <-].
-rewrite to_hoare_requestE;
-  apply/(doors_toggle_preE ω d)=>//.
+  rewrite to_hoare_when_preE // to_hoare_trigger_postE
+    => -[ /[swap] ]=>/doors_o_callee_is_openE ? ->.
+rewrite /= to_hoare_trigger_preE;
+  apply: req_toggle=>//.
 by move: safe=> /[swap] ->.
 Qed.
 
 Lemma close_door_run (ω : Ω) (d : door) (ω' : Ω) (x : unit)
-  (run : post (close_door d ||> doors_c) ω x ω') :
+  (run : post (doors_c ||> close_door d) ω x ω') :
 ~~ sel d ω'.
 Proof.
-move: run; rewrite /close_door th_post_bindA.
-move=> [opened [? [ ]]].
-rewrite to_hoare_requestE doors_is_open_post_retE to_hoare_when_postE
-  => -[+ <-].
-case: opened=> [ + [[]] | /[swap] -> -> ] //.
-by rewrite to_hoare_requestE doors_toggle_postE
-  => /[swap] ->;
-  rewrite tog_equ_1=> ->.
+move: run; rewrite /close_door th_post_bindA;
+  move=> [opened [? [ ] ] ];
+  rewrite to_hoare_trigger_postE /=;
+  rewrite to_hoare_when_postE=> -[<-] //;
+  case: opened=> /doors_o_callee_is_openE=> [H' [?] | /[swap] <- ->] //.
+by rewrite to_hoare_trigger_postE /= => -[-> _];
+  rewrite tog_equ_1 H'.
 Qed.
 
 Opaque close_door.
@@ -305,13 +213,13 @@ Opaque Nat.ltb.
 Opaque sel.
 
 Lemma doors_request_preserves_safe
-    `(op : Fx a) (ω : Ω) (x : a) (ω' : Ω) :
-  pre (trigger op ||> doors_c) ω ->
-  post (trigger op ||> doors_c) ω x ω' ->
+    {a : Type} (op : Fx a) (ω : Ω) (x : a) (ω' : Ω) :
+  pre (doors_c ||> trigger op) ω ->
+  post (doors_c ||> trigger op) ω x ω' ->
   doors_safe ω -> doors_safe ω'.
 Proof.
-rewrite to_hoare_requestE doors_effect_preE doors_effect_postE.
-case: (proj_p op)=> [door_op |] /=; last first.
+rewrite to_hoare_request_preE to_hoare_request_postE.
+case: (proj op)=> [door_op |] /=; last first.
 - by move=> _ ->.
 move=> + [-> _].
 move: door_op x; case=> d [] caller safe //=.
@@ -323,52 +231,48 @@ by inversion caller as [|?? Hsafe]; subst;
   move: co_open Hsafe d_closed=> -> ->.
 Qed.
 
-Lemma doors_handler_preserves_safe `(op : Fx a) :
+Lemma doors_handler_preserves_safe {a : Type} (op : Fx a) :
   preserves_invariant doors_safe (hoare_of_contract doors_c op).
 Proof.
-move=> ??? Hpre Hpost; apply/doors_request_preserves_safe ;
+move=> ??? Hpre Hpost.
+apply: doors_request_preserves_safe;
   rewrite to_hoare_requestE.
 - exact: Hpre.
 - exact: Hpost.
 Qed.
-
-(** /!\ WARNING: This proof exits the Equational Reasoning.
-  * This is a known issue. I need to find a way to remove this
-  * induction but can't find one right now.
-  *)
-Lemma doors_run_preserves_safe `(p : freer Fx A) :
-  preserves_invariant doors_safe (p |> doors_c).
-Proof.
-elim: p=> [value | X op k IH].
-- exact: preserves_invariant_ret.
-by apply: preserves_invariant_bind=>//;
-  exact: doors_handler_preserves_safe.
-Qed.
-
-Lemma respectful_run_inv `(p : im A)
-    (ω : Ω) (safe : ~~ sel left ω \/ ~~ sel right ω)
-    (a : A) (ω' : Ω)
-    (hpre : pre (p |> doors_c) ω)
-    (hpost : post (p |> doors_c) ω a ω') :
-  ~~ sel left ω' \/ ~~ sel right ω'.
-Proof.
-by move: hpre hpost safe;
-  (** /!\ WARNING: Reifying bridge used here.
-    * This currently holds only with a known
-    * instance of FreerMonad being Freer (and
-    * not for all Freer Monads...).
-    *)
-  rewrite -ToHoareFreerBridge.to_hoare_reifyE;
-  exact: doors_run_preserves_safe.
-Qed.
 End RespectfulAndRunLemmas.
+
+(* From now on, proofs will use the inductive version. *)
+Section InvariantRunLemmas.
+Context {Fx : effect} `{DOORS -< Fx} {M : inductiveFreerMonad Fx}.
+
+(** /!\ WARNING: This lemma is the only one needing `f_ind`  because we
+  * require to "execute" the freer program in order to denote it and see
+  * if the invariant was preserved all along.
+  *)
+Lemma doors_run_preserves_safe {A : Type} (p : M A) :
+  preserves_invariant doors_safe (doors_c |> p).
+Proof.
+by apply: to_hoare_preserves_invariant=> *;
+  exact: (doors_handler_preserves_safe (M:=M)).
+Qed.
+
+Lemma respectful_run_inv {A : Type} (p : M A)
+    (ω : Ω) (safe : doors_safe ω)
+    (a : A) (ω' : Ω)
+    (hpre : pre (doors_c |> p) ω)
+    (hpost : post (doors_c |> p) ω a ω') :
+  doors_safe ω'.
+Proof. by move: hpre hpost safe; exact: doors_run_preserves_safe. Qed.
+End InvariantRunLemmas.
 
 (** ** Main Theorem *)
 Section controller_s.
-Context `{StrictProvide2 Fx DOORS (STORE nat)} {im : freerMonad Fx}.
+Context {Fx : effect} `{StrictProvide2 Fx DOORS (STORE nat)}
+  {M : inductiveFreerMonad Fx}.
 
-Lemma controller_pre `(op: CONTROLLER α) (ω : Ω)
-  : pre ((controller (im:=im) α op) |> doors_c) ω.
+Lemma controller_pre {α : Type} (op : CONTROLLER α) (ω : Ω)
+  : pre (doors_c |> controller (M:=M) α op) ω.
 Proof.
 case: op=> [|d].
 - (* Tick *) apply: th_pre_bindA.
@@ -389,7 +293,7 @@ case: op=> [|d].
 Qed.
 
 Theorem controller_correct
-  : correct_component controller (im:=im)
+  : correct_component controller (M:=M)
     (no_contract CONTROLLER) doors_c (fun=> doors_safe).
 Proof.
 move=>? ω ?? op _; split=> [|?? Hpost]; [exact: controller_pre|split=> //].
