theories/Component.v
@@ -4,17 +4,7 @@
 
 (* Copyright (C) 2018–2020 ANSSI *)
 
-Attributes deprecated(
-  note="This file will probably be removed or
-    largely reworked in later versions.").
-
-From FreerDPS Require Import Init.
-(* From ExtLib Require Import StateMonad. *)
-From FreerDPS Require Export Effect Semantics Freer.
-From FreerDPS Require Import Contract Hoare.
-From monae Require Import monad_lib.
-
-Generalizable All Variables.
+From FreerDPS Require Import Init Effect Freer Contract Hoare.
 
 (** * Definition *)
 
@@ -34,84 +24,18 @@ Generalizable All Variables.
     Thus, a component [c : component F E] is a polymorphic function which
     maps primitives of [F] to impure computations using [E]. *)
 
-Definition component (F E : effect) `{im : freerMonad E} : Type :=
-  forall (α : Type), F α -> im α.
+Definition component (F E : effect) `{M : freerMonad E} : Type :=
+  forall (α : Type), F α -> M α.
 
-Definition correct_component `{MayProvide Ex E} {im : freerMonad Ex}
-    `(c : component F Ex) `(cF : contract F ΩF)
-    `(cE : contract E ΩE) (pred : ΩF -> ΩE -> Prop) :
+Definition correct_component {Ex E F : effect} `{E -<? Ex} {M : freerMonad Ex}
+  {ΩF ΩE : Type}
+    (c : component F Ex) (cF : contract F ΩF)
+    (cE : contract E ΩE) (pred : ΩF -> ΩE -> Prop) :
   Prop :=
-  forall (ωF : ΩF) (ωE : ΩE) (init : pred ωF ωE)
-      `(op : F α) (o_caller : caller_obligation cF ωF op),
+  forall (ωF : ΩF) (ωE : ΩE) (init : pred ωF ωE) (α : Type)
+      (op : F α) (o_caller : caller_obligation cF ωF op),
     pre (to_hoare cE $ c α op) ωE /\
     forall (x : α) (ωE' : ΩE),
-      post (to_hoare (im:=im) cE (c α op)) ωE x ωE' ->
+      post (to_hoare (M:=M) cE (c α op)) ωE x ωE' ->
       callee_obligation cF ωF op x /\
       pred (witness_update cF ωF op x) ωE'.
-
-(** The similarity between FreeSpec components and operational semantics may be
-    confusing at first. The main difference between the two concepts is simple:
-    operational semantics are self-contained terms which can, alone, be used to
-    interpret impure computations of a given effect.  Components, on the
-    other hand, are not self-contained.  Without an operational semantics for
-    [E], we cannot use a component [c : component F E] to interpret an impure
-    computation using [F].
-
-    Given an initial semantics for [E], we can however derive an operational
-    semantics for [F] from a component [c]. *)
-
-(** * Semantics Derivation *)
-
-
-CoFixpoint derive_semantics {F E} {im : freerMonad E}
-    (c : component F E) (sem : semantics E) : semantics F :=
-  mk_semantics (fun a p =>
-                  let (res, next) := (to_state (α:=im) _ $ c a p) sem in
-                  (res, derive_semantics c next)).
-
-(** So, [semprod] on the one hand allows for composing operational semantics
-    horizontally, and [derive_semantics] allows for composing components
-    vertically.  Using these two operators, we can model a complete system in a
-    hierarchical and modular manner, by defining each of its components
-    independently, then composing them together with [semprod] and
-    [derive_semantics]. *)
-
-Definition bootstrap {F} {im : freerMonad eempty}
-    (c : component F eempty) : semantics F :=
-  derive_semantics (im:=im) c eempty_semantics.
-
-(** * In-place Primitives Handling *)
-
-(** The function [with_component] allows for locally providing an additional
-    effect [E] within an impure computation of type [freer Fx a]. The
-    primitives of [E] will be handled by impure computations, i.e., a component.
-    of type [c : compoment E Fx s]. *)
-Local Open Scope monae_scope.
-
-#[local]
-Fixpoint with_component_aux {Fx E α}
-(c : component
-       (im:=freer Fx)
-       E Fx)
-    (p : freer (Fx + E) α)
-  : freer Fx α :=
-  match p with
-  | pure x => pure x
-  | impure T (in_right op) k =>
-    c T op >>= fun res => with_component_aux c (k res)
-  | impure _ (in_left op) k =>
-    impure op (fun x => with_component_aux c (k x))
-  end.
-
-Definition with_component {Fx E α}
-  (initializer : freer Fx unit)
-  (c : component
-         (im:=freer Fx)
-         E Fx)
-  (finalizer : freer Fx unit)
-  (p : freer (Fx + E) α)
-  : freer Fx α :=
-  initializer >>
-  with_component_aux c p >>= fun res =>
-  finalizer >>
-  pure res.
