theories/Core.v
@@ -4,13 +4,12 @@
 
 (* Copyright (C) 2018–2020 ANSSI *)
 
-From FreerDPS Require Import Init.
 From FreerDPS Require Export
-     Effect
-     Typeclasses
-     Freer
-     Semantics
-     Component
-     Contract
-     Hoare
-     .
+  Init
+  Effect
+  Typeclasses
+  Freer
+  Component
+  Contract
+  Hoare
+  .
